Imp/signals.v
@@ -1,8 +1,15 @@
-From Imp Require Import header_extensible exp_ite exp_lam.
+From Imp Require Import header_extensible.
+(* Feature functors *)
+From Imp Require Import exp_ite exp_lam exp_mut exp_err.
+(* Interaction functors *)
+From Imp Require Import int_lam_err int_ite_err int_mut_err.
+
 
 Inductive exp : Type := 
     | In_exp_lam : exp_lam exp -> exp
     | In_exp_ite : exp_ite exp -> exp
+    | In_exp_mut : exp_mut exp -> exp
+    | In_exp_err : exp_err exp -> exp
 .
 
 
@@ -25,11 +32,33 @@ Proof.
     - intros x y H. destruct y; (try easy).
       inversion H. easy.
 Defined.
+
+#[refine] Global Instance retract_exp_exp_mut : retract (exp_mut exp) exp := { 
+    retract_I := In_exp_mut; 
+    retract_R := fun x => match x with In_exp_mut t => Some t | _ => None end 
+    }.
+Proof.
+    - intros x. easy.
+    - intros x y H. destruct y; (try easy).
+      inversion H. easy.
+Defined.
+
+#[refine] Global Instance retract_exp_exp_err : retract (exp_err exp) exp := { 
+    retract_I := In_exp_err; 
+    retract_R := fun x => match x with In_exp_err t => Some t | _ => None end 
+    }.
+Proof.
+    - intros x. easy.
+    - intros x y H. destruct y; (try easy).
+      inversion H. easy.
+Defined.
     
 Fixpoint open_rec (k : nat) (u : exp) (e : exp) : exp := 
     match e with 
         | In_exp_lam e => open_rec_lam _ open_rec k u e
         | In_exp_ite e => open_rec_ite _ open_rec k u e
+        | In_exp_mut e => open_rec_mut _ open_rec k u e
+        | In_exp_err e => open_rec_err _ open_rec k u e
     end
 .
 
@@ -38,12 +67,16 @@ Fixpoint open_rec (k : nat) (u : exp) (e : exp) : exp :=
 Inductive lc' : nat -> exp -> Prop := 
     | lc_in_lam n e : lc'_lam _ lc' n e -> lc' n e
     | lc_in_ite n e : lc'_ite _ lc' n e -> lc' n e
+    | lc_in_mut n e : lc'_mut _ lc' n e -> lc' n e
+    | lc_in_err n e : lc'_err _ lc' n e -> lc' n e
 .
 
 
 Inductive value : exp -> Prop := 
     | value_in_lam (e : exp) : value_lam _ lc' e -> value e
     | value_in_ite (e : exp) : value_ite _ e -> value e
+    | value_in_mut (e : exp) : value_mut _ e -> value e
+    | value_in_err (e : exp) : value_err _ e -> value e
 .
 
 
@@ -51,28 +84,52 @@ Definition retract_lc_rev_ite : forall (n : nat) (e : exp_ite exp),
             lc' n (inj e) -> lc'_ite exp lc' n (inj e).
 Proof.
     intros n e.
-    inversion 1; subst; easy.
+    inversion 1; easy.
 Qed.
 
 Definition retract_lc_rev_lam : forall (n : nat) (e : exp_lam exp),
         lc' n (inj e) -> lc'_lam exp lc' n (inj e).
 Proof.
     intros n e.
-    inversion 1; subst; easy.
+    inversion 1; easy.
+Qed.
+
+Definition retract_lc_rev_mut : forall (n : nat) (e : exp_mut exp),
+        lc' n (inj e) -> lc'_mut exp lc' n (inj e).
+Proof.
+    intros n e.
+    inversion 1; easy.
+Qed.
+
+Definition retract_lc_rev_err : forall (n : nat) (e : exp_err exp),
+        lc' n (inj e) -> lc'_err exp lc' n (inj e).
+Proof.
+    intros n e.
+    inversion 1; easy.
 Qed.
 
 Definition retract_open_rec_rev_lam : forall (n : nat) s (e : exp_lam exp),
             open_rec n s (inj e) = open_rec_lam _ open_rec n s e.
 Proof.
-    intros n s e.
-    simpl. easy.
+    intros n s e. easy.
 Qed.
 
 Definition retract_open_rec_rev_ite : forall (n : nat) s (e : exp_ite exp),
             open_rec n s (inj e) = open_rec_ite _ open_rec n s e.
 Proof.
-    intros n s e.
-    simpl. easy.
+    intros n s e. easy.
+Qed.
+
+Definition retract_open_rec_rev_mut : forall (n : nat) s (e : exp_mut exp),
+            open_rec n s (inj e) = open_rec_mut _ open_rec n s e.
+Proof.
+    intros n s e. easy.
+Qed.
+
+Definition retract_open_rec_rev_err : forall (n : nat) s (e : exp_err exp),
+            open_rec n s (inj e) = open_rec_err _ open_rec n s e.
+Proof.
+    intros n s e. easy.
 Qed.
 
 Fixpoint lc_weaken   : forall s n m, n <= m -> lc' n s -> lc' m s.
@@ -80,6 +137,8 @@ intros s n m n_le_m Hlc.
 inversion Hlc; subst.
 - apply (lc_weaken_lam exp _ lc_weaken lc_in_lam _) with (n := n); easy.
 - apply (lc_weaken_ite exp _ lc_weaken lc_in_ite _) with (n := n); easy.
+- apply (lc_weaken_mut exp _ lc_weaken lc_in_mut _) with (n := n); easy.
+- apply (lc_weaken_err exp _ lc_weaken lc_in_err _) with (n := n); easy.
 Qed.
 
 Fixpoint open_rec_lc : forall s t n, lc' 0 s -> lc' (S n) t -> lc' n (open_rec n s t).
@@ -88,42 +147,161 @@ intros s t n H1 H2.
 inversion H2; subst.
 - apply (open_rec_lc_lam exp open_rec retract_open_rec_rev_lam lc' open_rec_lc lc_weaken lc_in_lam); easy.
 - apply (open_rec_lc_ite exp open_rec retract_open_rec_rev_ite lc' open_rec_lc lc_in_ite); easy.
+- apply (open_rec_lc_mut exp open_rec retract_open_rec_rev_mut lc' open_rec_lc lc_in_mut); easy.
+- apply (open_rec_lc_err exp open_rec retract_open_rec_rev_err lc' open_rec_lc lc_in_err); easy.
 Qed.
 
+Fixpoint value_lc : forall v, value v -> lc' 0 v.
+Proof.
+    intros v. induction 1.
+    - apply (value_lc_lam _ _); easy.
+    - apply (value_lc_ite _ _ lc_in_ite); easy.
+    - apply (value_lc_mut _ _ lc_in_mut); easy.
+    - apply (value_lc_err _ _); easy.
+Qed.
+
+Inductive tag := 
+    | In_tag_lam : tag_lam -> tag
+    | In_tag_ite : tag_ite -> tag
+    | In_tag_mut : tag_mut -> tag
+    | In_tag_err : tag_err -> tag
+.
+
+#[refine] Global Instance retract_tag_tag_ite : retract tag_ite tag := { 
+    retract_I := In_tag_ite; 
+    retract_R := fun x => match x with In_tag_ite t => Some t | _ => None end 
+    }.
+Proof.
+    - intros. reflexivity.
+    - intros x y. destruct y; try easy.
+      inversion 1. congruence.
+Defined.
+
+#[refine] Global Instance retract_tag_tag_lam : retract tag_lam tag := { 
+    retract_I := In_tag_lam; 
+    retract_R := fun x => match x with In_tag_lam t => Some t | _ => None end 
+    }.
+Proof.
+    - intros. reflexivity.
+    - intros x y. destruct y; try easy.
+      inversion 1. congruence.
+Defined.
+
+#[refine] Global Instance retract_tag_tag_mut : retract tag_mut tag := { 
+    retract_I := In_tag_mut; 
+    retract_R := fun x => match x with In_tag_mut t => Some t | _ => None end 
+    }.
+Proof.
+    - intros. reflexivity.
+    - intros x y. destruct y; try easy.
+      inversion 1. congruence.
+Defined.
+
+#[refine] Global Instance retract_tag_tag_err : retract tag_err tag := { 
+    retract_I := In_tag_err; 
+    retract_R := fun x => match x with In_tag_err t => Some t | _ => None end 
+    }.
+Proof.
+    - intros. reflexivity.
+    - intros x y. destruct y; easy.
+Defined.
+
+Inductive tag_of : exp -> tag -> Prop := 
+    | tag_of_in_lam e t: tag_of_lam _ _ e t -> tag_of e t
+    | tag_of_in_ite e t: tag_of_ite _ _ e t -> tag_of e t
+    | tag_of_in_mut e t: tag_of_mut _ _ e t -> tag_of e t
+    | tag_of_in_err e t: tag_of_err _ _ e t -> tag_of e t 
+.
+
+Lemma retract_tag_of_lam : forall (t : tag_lam) (e : exp_lam exp), tag_of (inj e) (inj t) <-> tag_of_lam _ _ (inj e) (inj t).
+Proof.
+    intros t e.
+    split.
+    - inversion 1; easy.
+    - constructor; easy.
+Qed.
+
+Lemma retract_tag_of_ite : forall (t : tag_ite) (e : exp_ite exp), tag_of (inj e) (inj t) <-> tag_of_ite _ _ (inj e) (inj t).
+Proof.
+    intros t e.
+    split.
+    - inversion 1; easy.
+    - constructor; easy.
+Qed.
+
+Lemma retract_tag_of_mut: forall (t : tag_mut) (e : exp_mut exp), tag_of (inj e) (inj t) <-> tag_of_mut _ _ (inj e) (inj t).
+Proof.
+    intros t e.
+    split.
+    - inversion 1; easy.
+    - constructor; easy.
+Qed.
+
+Lemma retract_tag_of_err : forall (t : tag_err) (e : exp_err exp), tag_of (inj e) (inj t) <-> tag_of_err _ _ (inj e) (inj t).
+Proof.
+    intros t e.
+    split.
+    - inversion 1; easy.
+    - constructor; easy.
+Qed.
+
+Lemma tag_of_decidable e t : ~tag_of e t \/ tag_of e t.
+Proof.
+    destruct e; destruct t.
+    all: try (rewrite retract_tag_of_lam; apply tag_of_decidable_lam).
+    all: try (rewrite retract_tag_of_ite; apply tag_of_decidable_ite).
+    all: try (rewrite retract_tag_of_mut; apply tag_of_decidable_mut).
+    all: try (rewrite retract_tag_of_mut; apply tag_of_decidable_mut).
+    all: try (rewrite retract_tag_of_err; apply tag_of_decidable_err).
+    all: left; inversion 1; inversion H0.
+Qed.
 
 From Imp Require Import context.
 
-Module SIGNALS (Import Atom : ATOM) (Import String : STRING).
+Definition VarEnv := Env (sig value).
 
-    Module Import Env := Imp.context.Env (Atom) (String).
+Record Ctx := mkCtx {
+        store : VarEnv;
+}.
 
-    Inductive stored_val : Type := val_with_proof : forall (v : exp), value v -> stored_val.
+#[refine] Global Instance ctx_supports_store : hasProj Ctx VarEnv := {
+    get_proj := store;
+    set_proj := (fun x c => mkCtx x);
+}.
+Proof.
+    - intros. easy.
+    - intros. destruct c. simpl. easy.
+Defined.
 
-    Record Ctx := mkCtx {
-        store : Env.AtomEnv.t stored_val;
-    }.
+Inductive step : Ctx -> exp -> Ctx -> exp -> Prop := 
+    | step_in_lam (c : Ctx) s c' s' : step_lam _ open_rec value _ step c s c' s' -> step c s c' s'
+    | step_in_ite (c : Ctx) s c' s' : step_ite _ _                step c s c' s' -> step c s c' s'
+    | step_in_mut (c : Ctx) s c' s' : step_mut _ _ _              step c s c' s' -> step c s c' s'
+    | step_in_err (c : Ctx) s c' s' : step_err _ _                step c s c' s' -> step c s c' s'
+    (* interactions *)
+    | step_in_lam_err (c : Ctx) s c' s' : step_int_lam_err _ value _ tag_of _ step c s c' s' -> step c s c' s'
+    | step_in_ite_err (c : Ctx) s c' s' : step_int_ite_err _ value _ tag_of _ step c s c' s' -> step c s c' s'
+    | step_in_mut_err (c : Ctx) s c' s' : step_int_mut_err _ value _ tag_of _ step c s c' s' -> step c s c' s'
+.
 
-    Inductive step : Ctx -> exp -> Ctx -> exp -> Prop := 
-        | step_in_lam (c : Ctx) s c' s' : step_lam _ open_rec value _ step c s c' s' -> step c s c' s'
-        | step_in_ite (c : Ctx) s c' s' : step_ite _ _ step c s c' s'                -> step c s c' s'
-    .
+Definition lc := lc' 0.
+Definition open := open_rec 0.
 
-    Definition lc := lc' 0.
-    Definition open := open_rec 0.
-
-
-    Fixpoint preservation : forall c e c' e', 
+Fixpoint preservation : forall c e c' e', 
     lc e -> 
     step c e c' e' -> 
     lc e'. 
-    Proof. 
-        intros c e c' e'.
-        unfold lc in *.
-        induction 2.
-        - apply (preservation_lam exp open_rec lc' open_rec_lc lc_in_lam retract_lc_rev_lam value Ctx step preservation c s c' s'); easy.
-        - apply (preservation_ite exp lc' lc_in_ite retract_lc_rev_ite Ctx step preservation c s c' s'); easy.
-    Defined.
-
-End SIGNALS.
-
+Proof. 
+    intros c e c' e'.
+    unfold lc in *.
+    induction 2.
+    - apply (preservation_lam exp open_rec lc' open_rec_lc lc_in_lam retract_lc_rev_lam value Ctx step preservation c s c' s'); easy.
+    - apply (preservation_ite exp lc' lc_in_ite retract_lc_rev_ite Ctx step preservation c s c' s'); easy.
+    - apply (preservation_mut exp lc' lc_in_mut retract_lc_rev_mut value value_lc Ctx step preservation c s c' s'); easy.
+    - apply (preservation_err exp lc' lc_in_err retract_lc_rev_err Ctx step preservation c s c' s'); easy.
+    (* interactions *)
+    - apply (preservation_lam_err exp lc' lc_in_err retract_lc_rev_lam retract_lc_rev_err value value_lc tag tag_of Ctx step preservation c s c' s'); easy.
+    - apply (preservation_ite_err exp lc' lc_in_err retract_lc_rev_ite retract_lc_rev_err value value_lc tag tag_of Ctx step preservation c s c' s'); easy.
+    - apply (preservation_mut_err exp lc' lc_in_mut lc_in_err retract_lc_rev_mut value tag tag_of Ctx step preservation c s c' s'); easy.
+Defined.
 
